src/Appraisal_Evidence.v
@@ -1,4 +1,4 @@
-Require Import ConcreteEvidence AutoApp Auto Helpers_CvmSemantics Term_Defs Anno_Term_Defs Cvm_St Cvm_Impl Defs StructTactics OptMonad_Coq IO_Stubs Evidence_Bundlers. (* Cvm_Monad. *)
+Require Import ConcreteEvidence AutoApp Auto Helpers_CvmSemantics Term_Defs Anno_Term_Defs Cvm_St Cvm_Impl Defs StructTactics OptMonad_Coq IO_Stubs Evidence_Bundlers Axioms_Io External_Facts. (* Cvm_Monad *)
 
 Require Import List.
 Import ListNotations.
@@ -72,6 +72,7 @@ Fixpoint encodeEv (e:EvidenceC) : RawEv :=
   | hhc _ _ bs _ => [bs]
   | eec _ _ bs _ => [bs]
   | kkc _ _ _ => []
+  | kpc _ _ e' => encodeEv e'
   | ssc e1 e2 => (encodeEv e1) ++ (encodeEv e2)
   end.
 
@@ -105,7 +106,9 @@ Fixpoint reconstruct_ev' (ls:RawEv) (et:Evidence) : Opt EvidenceC :=
       | [] => Some (kkc p ps et')
       | _ => None
       end
-    | KEEP => None
+    | KEEP =>
+      x <- reconstruct_ev' ls et' ;;
+      Some (kpc p ps x)
     end
   | nn i =>
     '(bs, ls') <- peel_bs ls ;;
@@ -132,7 +135,8 @@ Inductive reconstruct_evP: EvC -> EvidenceC -> Prop :=
 
 Lemma inv_recon_mt: forall ls et,
     reconstruct_evP (evc ls et) mtc ->
-    (et = mt \/ exists p ps et', et = uu p KILL ps et').
+    (et = mt) (* \/ (exists p ps et', et = uu p KILL ps et')
+    \/ (exists p ps et', et = uu p KEEP ps et')) *) .
 Proof.
   intros.
   invc H.
@@ -144,7 +148,12 @@ Proof.
                     
          -
            eauto.
-                                 
+           (*
+         -
+           right.
+           right.
+           eauto. *)
+                                   
 Defined.
 
 Ltac do_inv_recon_mt :=
@@ -152,9 +161,9 @@ Ltac do_inv_recon_mt :=
   | [H: reconstruct_evP (evc _ ?et) mtc
 
      |- _] =>
-    assert_new_proof_by (et = mt \/ exists p ps et', et = uu p KILL ps et') ltac:(eapply inv_recon_mt; apply H)
+    assert_new_proof_by (et = mt (* \/ (exists p ps et', et = uu p KILL ps et') \/ (exists p ps et', et = uu p KEEP ps et') *) ) ltac:(eapply inv_recon_mt; apply H)
   end;
-  door;
+  (* door; *)
   subst.
 
 Lemma inv_recon_mt': forall ls e,
@@ -178,11 +187,19 @@ Ltac do_inv_recon_mt' :=
 
 Lemma inv_recon_nn: forall ls et n n0,
     reconstruct_evP (evc ls et) (nnc n n0) ->
-    et = nn n /\ ls = [n0].
+    ((et = nn n /\ ls = [n0]) (* \/ (exists p ps et', et = uu p KEEP ps et') *) ).
 Proof.
   intros.
   invc H.
   destruct et; repeat ff; try (unfold OptMonad_Coq.bind in *); repeat ff; destruct ls; try solve_by_inversion.
+
+                               (*
+                               -
+                                 eauto.
+                               -
+                                 eauto. *)
+                                 
+                                 
 Defined.
 
 Ltac do_inv_recon_nn :=
@@ -190,7 +207,7 @@ Ltac do_inv_recon_nn :=
   | [H: reconstruct_evP (evc ?ls ?et) (nnc ?n ?nval)
 
      |- _] =>
-    assert_new_proof_by (et = nn n /\ ls = [nval]) ltac:(eapply inv_recon_nn; apply H)
+    assert_new_proof_by (et = nn n /\ ls = [nval] (* \/ (exists p ps et', et = uu p KEEP ps et') *) ) ltac:(eapply inv_recon_nn; apply H)
   end;
   destruct_conjs;
   subst.
@@ -198,14 +215,21 @@ Ltac do_inv_recon_nn :=
 Lemma inv_recon_gg: forall p ps ls et n ec,
     reconstruct_evP (evc ls et) (ggc p ps n ec) ->
     (exists ls' et', et = uu p EXTD ps et' /\
-                ls = n :: ls').
+                ls = n :: ls') (* \/ (exists p ps et', et = uu p KEEP ps et') *) .
 Proof.
   intros.
   invc H.
   destruct et; repeat ff; try (unfold OptMonad_Coq.bind in *); repeat ff; try solve_by_inversion.
-
-  repeat eexists.
-  destruct ls; ff.
+                               -
+                                 (*
+                                 left. *)
+                                 repeat eexists.
+                                 destruct ls; ff.
+                                 (*
+                               -
+                                 right.
+                                 eauto. *)
+                                 
 Defined.
 
 Ltac do_inv_recon_gg :=
@@ -213,8 +237,8 @@ Ltac do_inv_recon_gg :=
   | [H: reconstruct_evP (evc ?ls ?et) (ggc ?p ?ps ?n _)
 
      |- _] =>
-    assert_new_proof_by (exists ls' et', et = uu p EXTD ps et' /\
-                                    ls = n :: ls')
+    assert_new_proof_by ((exists ls' et', et = uu p EXTD ps et' /\
+                                    ls = n :: ls') (* \/ (exists p ps et', et = uu p KEEP ps et') *) )
                         ltac:(eapply inv_recon_gg; apply H)
   end;
   destruct_conjs;
@@ -222,11 +246,18 @@ Ltac do_inv_recon_gg :=
 
 Lemma inv_recon_hh: forall p ps ls et n et',
     reconstruct_evP (evc ls et) (hhc p ps n et') ->
-    (et = uu p COMP ps et' ) /\ ls = [n].
+    ((et = uu p COMP ps et' ) /\ ls = [n]) (* \/ (exists p ps et', et = uu p KEEP ps et') *) .
 Proof.
   intros.
   invc H.
   destruct et; repeat ff; try (unfold OptMonad_Coq.bind in *); repeat ff; destruct ls; try solve_by_inversion.
+                               (*
+                               -
+                                 right. eauto.
+                               -
+                                 right. eauto. *)
+                                 
+                                 
 Defined.
 
 Ltac do_inv_recon_hh :=
@@ -234,7 +265,7 @@ Ltac do_inv_recon_hh :=
   | [H: reconstruct_evP (evc ?ls ?et) (hhc ?p ?ps ?hval ?et')
 
      |- _] =>
-    assert_new_proof_by (et = uu p COMP ps et' /\ ls = [hval])
+    assert_new_proof_by ((et = uu p COMP ps et' /\ ls = [hval]) (* \/ (exists p ps et', et = uu p KEEP ps et') *) )
                         ltac:(eapply inv_recon_hh; apply H)
   end;
   destruct_conjs;
@@ -243,15 +274,23 @@ Ltac do_inv_recon_hh :=
 Lemma inv_recon_ee: forall p ps ls et (*et'*) n ec',
     reconstruct_evP (evc ls et) (eec p ps n (*et'*) ec') ->
     (* (exists et', et = uu p ENCR ps et' ) /\ ls = [n]. *)
-    (exists et', et = uu p ENCR ps et' /\ ls = [n]).
+    (exists et', et = uu p ENCR ps et' /\ ls = [n]) (* \/ (exists p ps et', et = uu p KEEP ps et') *) .
 Proof.
   intros.
   invc H.
   destruct et; repeat ff; try (unfold OptMonad_Coq.bind in *); repeat ff; destruct ls; try solve_by_inversion.
                                -
-                               ff.
+                                 (*
+                                 left. *)
                                repeat eexists.
                                ff.
+                               (*
+                               -
+                                 right. eauto.
+                               -
+                                 right. eauto. *)
+                                 
+                                 
                                
 Defined.
 
@@ -260,7 +299,7 @@ Ltac do_inv_recon_ee :=
   | [H: reconstruct_evP (evc ?ls ?et) (eec ?p ?ps ?hval (*_*) _)
 
      |- _] =>
-    assert_new_proof_by (exists et', et = uu p ENCR ps et' /\ ls = [hval])
+    assert_new_proof_by ( (exists et', et = uu p ENCR ps et' /\ ls = [hval]) (* \/ (exists p ps et', et = uu p KEEP ps et') *) )
                         ltac:(eapply inv_recon_ee; apply H)
   end;
   destruct_conjs;
@@ -290,12 +329,19 @@ Ltac do_inv_recon_kk :=
 
 Lemma inv_recon_ss: forall ls et ec1 ec2,
     reconstruct_evP (evc ls et) (ssc ec1 ec2) ->
-    (exists et1 et2, et = ss et1 et2).
+    (exists et1 et2, et = ss et1 et2) (* \/ (exists p ps et', et = uu p KEEP ps et') *) .
 Proof.
   intros.
   invc H.
   destruct et; repeat ff; try (unfold OptMonad_Coq.bind in *); repeat ff; try solve_by_inversion.
-  eauto.
+                               -
+                                 (*
+                                 right. *)  eauto.
+                                            (* 
+                               -
+                               left. eauto.
+                                             *)
+                                            
 Defined.
 
 Ltac do_inv_recon_ss :=
@@ -303,7 +349,7 @@ Ltac do_inv_recon_ss :=
   | [H: reconstruct_evP (evc _ ?et) (ssc _ _)
 
      |- _] =>
-    assert_new_proof_by (exists et1 et2, et = ss et1 et2)
+    assert_new_proof_by ((exists et1 et2, et = ss et1 et2) (* \/ (exists p ps et', et = uu p KEEP ps et') *) )
                         ltac:(eapply inv_recon_ss; apply H)
   end;
   destruct_conjs;
@@ -361,7 +407,7 @@ Ltac do_recon_inv_ss :=
   match goal with
   | [H: reconstruct_evP
           (evc ?ls (ss ?H1 ?H2))
-          (ssc ?ec1 ?ec2)
+          (ssc ?ec1 ?ec2) _
      |- _] =>
     assert_new_proof_by
       (reconstruct_evP (evc (firstn (et_size H1) ls) H1) ec1 /\
@@ -415,7 +461,7 @@ TODO: try this again after appraisal lemmas settled
 
 Lemma etfun_reconstruct: forall e e0 e1,
     reconstruct_evP (evc e0 e1) e ->
-    e1 = et_fun e.
+    e1 = et_fun e (* \/ (exists p ps et', e1 = uu p KEEP ps et' /\ et' = et_fun e) *) .
 Proof.
   intros.
   generalizeEverythingElse e1.
@@ -474,7 +520,19 @@ Proof.
 
 
   
-  induction e1; intros e e0 H;
+  induction e1; intros e e0 H.
+  - (* mt case *)
+    invc H.
+    ff.
+    tauto.
+  - (* nn case *)
+    invc H.
+    repeat ff; try (unfold OptMonad_Coq.bind in * ); repeat ff.
+    
+    
+    
+
+  (* 
     try (
     do_inv_recon;
     ff;
@@ -483,9 +541,9 @@ Proof.
     rewrite fold_recev in *;
     do_wrap_reconP;
     repeat jkjke).
-
-  (*
-  -
+   *)
+  
+  - (* uu case *)
     destruct f; ff.
     + (* COMP case *)
       invc H.
@@ -503,24 +561,69 @@ Proof.
       unfold reconstruct_ev' in *.
       unfold OptMonad_Coq.bind in *.
       repeat ff; try (unfold OptMonad_Coq.bind in * ); repeat ff.
+           
     + (* EXTD case *)
+      (* left. *)
       invc H.
       ff.
       repeat ff; try (unfold OptMonad_Coq.bind in * ); repeat ff.
-      assert (e1 = et_fun e2).
+      assert (e1 = et_fun e2 (* \/ (exists (p : Plc) (ps : ASP_PARAMS) (et' : Evidence),
+                                   e1 = uu p KEEP ps et' /\ et' = et_fun e2) *) ).
+      {
       eapply IHe1.
       econstructor.
       ff.
+      }
+      (*
+      door.
+      ++ *)
+        
       congruence.
+      (*
+      ++
+        
+        
+      subst.
+      
+      
+      congruence. *)
     + (* KILL case *)
       invc H.
       unfold reconstruct_ev in *.
-     
-      Print et_fun.
       ff.
+    + (* KEEP case *)
+      invc H.
+      unfold reconstruct_ev in *.
       ff.
-      
-*)
+      repeat ff; try (unfold OptMonad_Coq.bind in * ); repeat ff.
+      assert (e1 = et_fun e2).
+      { eapply IHe1.
+        econstructor.
+        unfold reconstruct_ev.
+        symmetry.
+        eassumption.
+      }
+      subst.
+      tauto.
+  - (* ss case *)
+    invc H.
+    ff.
+    repeat ff; try (unfold OptMonad_Coq.bind in * ); repeat ff.
+    assert (e1_1 = et_fun e1).
+    {
+      eapply IHe1_1.
+      econstructor.
+      symmetry.
+      eassumption.
+    }
+    assert (e1_2 = et_fun e2).
+    {
+      eapply IHe1_2.
+      econstructor.
+      symmetry.
+      eassumption.
+    }
+    congruence.
 Qed.
 
 Lemma wfec_split: forall e s,
@@ -562,8 +665,9 @@ Proof.
     do_inv_recon.
     invc H.
     repeat ff.
+    (*
     invc H.
-    repeat ff.
+    repeat ff. *)
   - (* nnc case *)
     do_inv_recon.
     ff.
@@ -604,8 +708,58 @@ Proof.
     unfold OptMonad_Coq.bind in *.
     ff.
     rewrite fold_recev in *.
-    do_wrap_reconP.
-    admit.
+    unfold reconstruct_ev in *.
+    unfold reconstruct_ev' in *.
+    destruct et; try solve_by_inversion.
+    ff.
+    unfold OptMonad_Coq.bind in *.
+    ff.
+    unfold OptMonad_Coq.bind in *.
+    ff.
+    unfold OptMonad_Coq.bind in *.
+    ff.
+
+
+  - (* kpc case *)
+    ff.
+
+    assert (exists et', et = uu p KEEP a et').
+    {
+      destruct et; try solve_by_inversion.
+      +
+        invc H.
+        ff.
+      +
+        invc H.
+        ff.
+        repeat ff; try (unfold OptMonad_Coq.bind in * ); repeat ff.
+      +
+        invc H.
+        ff.
+        repeat ff; try (unfold OptMonad_Coq.bind in * ); repeat ff.
+        repeat ff; try (unfold OptMonad_Coq.bind in * ); repeat ff.
+        repeat ff; try (unfold OptMonad_Coq.bind in * ); repeat ff.
+        repeat ff; try (unfold OptMonad_Coq.bind in * ); repeat ff.
+        eexists.
+        tauto.
+      +
+        invc H.
+        ff.
+        repeat ff; try (unfold OptMonad_Coq.bind in * ); repeat ff.
+    }
+    
+    destruct_conjs.
+    subst.
+
+    invc H.
+    ff.
+    repeat ff; try (unfold OptMonad_Coq.bind in * ); repeat ff.
+    eapply IHec.
+    econstructor.
+    ff.
+    
+    
+    
     
     
     
@@ -630,7 +784,7 @@ Proof.
     }
     rewrite H3 at 1.
     congruence.
-Admitted.
+Qed.
 
 Lemma recon_encodeEv_Raw: forall ec bits et,
     reconstruct_evP (evc bits et) ec ->
@@ -650,23 +804,24 @@ Proof.
   intros.
   generalizeEverythingElse ec.
   induction ec; intros; destruct ee.
-  -
+  - (* mtc case *)
     do_inv_recon.
     dd.
     invc H.
     dd.
     ff.
     econstructor. tauto.
+    (* 
     invc H.
-    repeat ff.
+    repeat ff. *)
     (*
     econstructor. tauto. *)
-  -
+  - (* nnc case *)
     do_inv_recon.
     invc H.
     dd.
     econstructor; tauto.
-  -
+  - (* ggc case *)
     do_inv_recon.
     invc H.
     dd.
@@ -684,12 +839,12 @@ Proof.
     invc H.
     lia.
 
-  -
+  - (* hhc case *)
     do_inv_recon.
     invc H.
     dd.
     econstructor; tauto.
-  -
+  - (* eec case *)
     do_inv_recon.
     invc H.
     dd.
@@ -702,10 +857,36 @@ Proof.
      *)
 
   - (* kkc case *)
-    admit.
-    
-    
-    
+    invc H.
+    unfold reconstruct_ev in *.
+    unfold reconstruct_ev' in *.
+    destruct e0; try solve_by_inversion.
+    ff.
+    unfold OptMonad_Coq.bind in *. ff.
+    unfold OptMonad_Coq.bind in *. ff.
+    econstructor.
+    ff.
+    unfold OptMonad_Coq.bind in *. ff.
+  - (* kpc case *)
+    invc H.
+    destruct e; try solve_by_inversion.
+    +
+      ff.
+    +
+      ff.
+      repeat ff; try (unfold OptMonad_Coq.bind in * ); repeat ff.
+    +
+      repeat ff; try (unfold OptMonad_Coq.bind in * ); repeat ff.
+      assert (wf_ec (evc r e)).
+      {
+        eapply IHec. econstructor.
+        symmetry. eassumption. }
+      econstructor.
+      ff.
+    +
+      ff.
+      repeat ff; try (unfold OptMonad_Coq.bind in * ); repeat ff.
+   
   -
     do_inv_recon.
     invc H.
@@ -741,7 +922,7 @@ Proof.
     }
     rewrite H at 1.
     eapply app_length.
-Admitted.
+Qed.
 
 Lemma reconP_determ: forall ec e e',
     reconstruct_evP ec e ->
@@ -767,13 +948,41 @@ Ltac do_reconP_determ :=
 
 
 
+Ltac inv_wfec :=
+  repeat
+    match goal with
+    | [H: wf_ec _ |-  _ ] => invc H
+    end.
 
+(** * If a raw evidence sequence is non-empty, we can grab a first element. *)
+Lemma some_recons' : forall e x,
+    length e = S x ->
+    exists bs ls', peel_bs e = Some (bs, ls').
+Proof.
+  intros.
+  destruct e;
+    ff; eauto.
+Defined.
 
+Ltac do_some_recons' :=
+  match goal with
+  | [H: length ?e = S _ |- _ ] =>
+    edestruct some_recons'; [apply H | idtac]
+                              
+  end; destruct_conjs; jkjke.
 
+Ltac do_rcih :=
+  match goal with
+  | [H: context[reconstruct_ev' _ _]
+               
 
-
-(*
-
+     |- context[reconstruct_ev' ?e' ?et] ] =>
+    assert_new_proof_by
+      (exists x, Some x = reconstruct_ev' e' et)
+      ltac:(eapply H with (r:=e'); (* TODO:  make r less one-off *)
+            try (eapply peel_fact; eauto; tauto);
+            try (econstructor; first [eapply firstn_long | eapply skipn_long]; try eauto; try lia))      
+  end.
 
 (** * Lemma:  well-formed EvC bundles can be successfully reconstructed to a Typed Concrete Evidence (EvidenceC) value. *)
 Lemma some_recons : forall (e:EvC),
@@ -799,7 +1008,7 @@ Proof.
           repeat jkjke';
           repeat ff; eauto).
 
-  -
+  - (* nn case *)
     repeat ff.
     (unfold OptMonad_Coq.bind in * ).
      repeat ff.
@@ -822,13 +1031,113 @@ Proof.
 
 
     
-     -
+  - (* uu case *)
+
+    destruct f.
+    
+    + (* COMP case *)
+
+      inv_wfec.
+      ff.
+      repeat ff;
+    (unfold OptMonad_Coq.bind in * );
+    repeat ff; eauto.
+
+      ++
+       ff.
+       assert (exists v, r = [v]).
+       {
+         destruct r; ff.
+         destruct r; ff. }
+       destruct_conjs. subst.
+       ff.
+      ++
+       assert (exists v, r = [v]).
+       {
+         destruct r; ff. }
+       destruct_conjs. subst.
+       ff.
+    + (* ENCR case *)
+
+      inv_wfec.
+      ff.
+      repeat ff;
+    (unfold OptMonad_Coq.bind in * );
+    repeat ff; eauto.
+      ++
+         ff.
+       assert (exists v, r = [v]).
+       {
+         destruct r; ff.
+         destruct r; ff. }
+       destruct_conjs. subst.
+       ff.
+      ++
+       assert (exists v, r = [v]).
+       {
+         destruct r; ff. }
+       destruct_conjs. subst.
+       ff.
+    + (* EXTD case *)
+      inv_wfec.
+      ff.
+      unfold OptMonad_Coq.bind in * ;
+        repeat ff; eauto.
+      ++
+        assert (wf_ec (evc r0 e)).
+        {
+          eapply peel_fact.
+          eassumption.
+          eassumption.
+          tauto.
+        }
        
-       
-       
+          
+          
+        assert (exists ee, Some ee = reconstruct_ev' r0 e).
+        {
+          invc H.
+          eapply IHe.
+         econstructor. eassumption. }
+        destruct_conjs.
+        ff.
+      ++
+         inv_wfec.
+       ff.
+       assert (r = []).
+       {
+         destruct r; ff.
+       }
+       subst.
+       ff.
+    + (* KILL case *)
+      inv_wfec.
+      ff.
+      eauto.
+    + (* KEEP case *)
+      inv_wfec.
+      simpl in H1.
+      ff.
+
     repeat ff;
     (unfold OptMonad_Coq.bind in * );
-     repeat ff; eauto.
+    repeat ff; eauto.
+    assert (exists ee, Some ee = reconstruct_ev' r e).
+    { eapply IHe.
+      econstructor.
+      eassumption.
+    }
+    destruct_conjs.
+    congruence.
+
+
+
+
+    (*
+
+
+
+    
      +
        inv_wfec.
        ff.
@@ -891,6 +1200,7 @@ Proof.
        
        
        
+       
       (* 
        
        
@@ -942,7 +1252,7 @@ Proof.
        eassumption.
        asdf
        
-       
+       *)
          
        
     
@@ -979,7 +1289,6 @@ Ltac do_somerecons :=
         (exists x, reconstruct_evP e x)
         ltac:(eapply some_reconsP; apply H)     
     end; destruct_conjs.
-*)
 
 Definition spc_ev (sp:SP) (e:EvidenceC) : EvidenceC :=
   match sp with
@@ -1000,7 +1309,7 @@ Definition cvm_evidence_denote_asp (a:ASP) (p:Plc) (e:EvidenceC) (x:Event_ID): E
     | COMP => hhc p params (do_asp params (encodeEv (spc_ev sp e)) p x) (sp_ev sp (et_fun e))
     | EXTD => ggc p params (do_asp params (encodeEv (spc_ev sp e)) p x) (spc_ev sp e)
     | ENCR => eec p params (do_asp params (encodeEv (spc_ev sp e)) p x) (sp_ev sp (et_fun e)) (* (spc_ev sp e) (sp_ev sp (et_fun e)) *)
-    | KEEP => e
+    | KEEP => (spc_ev sp e)
     | KILL => mtc (* kkc p params (sp_ev sp (et_fun e)) *)
     end
   | SIG => ggc p sig_params (do_asp sig_params (encodeEv e) p x) e
@@ -1021,8 +1330,489 @@ Fixpoint cvm_evidence_denote (t:AnnoTerm) (p:Plc) (ec:EvidenceC) : EvidenceC :=
                          (cvm_evidence_denote t2 p ((splitEvr s ec)))
   end.
 
+
+(** * Assert an arbitrary (remote) CVM execution.  
+      Uses uninterpreted functions for "simulated" CVM evidence and events. *)
+Ltac do_assert_remote t e p i :=
+  assert (
+      build_cvm t
+                      {| st_ev := e; st_trace := []; st_pl := p; st_evid := i|} =
+      (Some tt,
+       {| st_ev := cvm_evidence_core t p e;
+                   st_trace := cvm_events_core t p (get_et e);
+                               st_pl := p; st_evid :=  (i + event_id_span t)
+       |})
+    ) by (eapply build_cvm_external).
+
+
+(*
+Ltac do_assume_remote t e p i (* x *) :=
+  (* do_t_at_zero t x; *)
+  do_assert_remote (*x*) t e p i (* ;
+  do_assert_unannoPar t x *) .
+ *)
+
+
+(**  * Event ID spans same for a term and its corresponding core term. *)
+Lemma event_id_spans_same : forall t,
+    event_id_span' t = event_id_span (copland_compile t).
+Proof.
+  intros.
+  induction t; ff.
+  -
+    destruct a; ff; try tauto.
+    (* 
+    +
+      destruct s; ff.
+  -
+    jkjke'.
+  -
+    destruct s0; ff; lia.
+  -
+    destruct s0; ff; lia. *)
+Qed.
+
+(** * Lemma:  CVM increases event IDs according to event_id_span' denotation. *)
+Lemma cvm_spans: forall t pt e tr p i e' tr' p' i',
+    term_to_coreP t pt ->
+    build_cvmP
+      pt
+      {| st_ev := e;
+         st_trace := tr;
+         st_pl := p;
+         st_evid := i |}
+      (Some tt)
+      {|
+        st_ev := e';
+        st_trace := tr';
+        st_pl := p';
+        st_evid := i'
+      |} ->
+    i' = i + event_id_span' t.
+Proof.
+  intros.
+  generalizeEverythingElse t.
+  induction t; intros;
+    wrap_ccp_anno.
+
+  
+ (*   (* This is more automated, but slower *)
+    try (
+        destruct a;
+        try destruct a;
+        ff; tauto);
+    try (
+        repeat find_apply_hyp_hyp;
+        lia).
+Defined.
+  *)
+   
+  -
+    destruct a;
+      try destruct a;
+      ff; try tauto.
+    +
+      wrap_ccp_anno; ff.
+    +
+      wrap_ccp_anno; ff.
+    +
+      destruct s.
+      ++
+        wrap_ccp_anno; ff.
+      ++
+        wrap_ccp_anno; ff.
+    +
+      wrap_ccp_anno; ff.
+    +
+      wrap_ccp_anno; ff.
+    +
+      wrap_ccp_anno; ff.
+    +
+      wrap_ccp_anno; ff.
+      
+      
+  
+  -
+    lia.
+  -
+    wrap_ccp_anno.
+    assert (st_evid0 = i + event_id_span' t1).
+    eapply IHt1.
+    2: { eassumption. }
+    econstructor; eauto.
+
+    assert (i' = st_evid0 + event_id_span' t2).
+    eapply IHt2.
+    2: { eassumption. }
+    econstructor; eauto.
+    lia.
+  -
+    destruct s0; destruct s1.
+    +
+      wrap_ccp_anno.
+
+      assert (st_evid1 = (i + 1) +  event_id_span' t1).
+    eapply IHt1.
+    2: { eassumption. }
+    econstructor; eauto.
+
+    assert (st_evid = st_evid1 + event_id_span' t2).
+    eapply IHt2.
+    2: { eassumption. }
+    econstructor; eauto.
+    subst.
+    lia.
+    +
+      wrap_ccp_anno.
+      assert (st_evid1 = (i + 1) +  event_id_span' t1).
+    eapply IHt1.
+    2: { eassumption. }
+    econstructor; eauto.
+
+    assert (st_evid = st_evid1 + event_id_span' t2).
+    eapply IHt2.
+    2: { eassumption. }
+    econstructor; eauto.
+    subst.
+    lia.
+    +
+      wrap_ccp_anno.
+      assert (st_evid1 = (i + 1) +  event_id_span' t1).
+    eapply IHt1.
+    2: { eassumption. }
+    econstructor; eauto.
+
+    assert (st_evid = st_evid1 + event_id_span' t2).
+    eapply IHt2.
+    2: { eassumption. }
+    econstructor; eauto.
+    subst.
+    lia.
+    +
+      wrap_ccp_anno.
+      assert (st_evid1 = (i + 1) +  event_id_span' t1).
+    eapply IHt1.
+    2: { eassumption. }
+    econstructor; eauto.
+
+    assert (st_evid = st_evid1 + event_id_span' t2).
+    eapply IHt2.
+    2: { eassumption. }
+    econstructor; eauto.
+    subst.
+    lia.
+  - (* bpar case *)
+    destruct s0; destruct s1.
+    +
+      wrap_ccp_anno.
+
+      assert (st_evid = (i + 1) +  event_id_span' t1).
+    eapply IHt1.
+    2: { eassumption. }
+    econstructor; eauto.
+
+    assert (event_id_span' t2 = event_id_span (copland_compile t2)).
+    {
+      eapply event_id_spans_same.
+    }
+    lia.
+    +
+      wrap_ccp_anno.
+
+      assert (st_evid = (i + 1) +  event_id_span' t1).
+    eapply IHt1.
+    2: { eassumption. }
+    econstructor; eauto.
+
+    assert (event_id_span' t2 = event_id_span (copland_compile t2)).
+    {
+      eapply event_id_spans_same.
+    }
+    lia.
+    +
+            wrap_ccp_anno.
+
+      assert (st_evid = (i + 1) +  event_id_span' t1).
+    eapply IHt1.
+    2: { eassumption. }
+    econstructor; eauto.
+
+    assert (event_id_span' t2 = event_id_span (copland_compile t2)).
+    {
+      eapply event_id_spans_same.
+    }
+    lia.
+    +
+      wrap_ccp_anno.
+
+      assert (st_evid = (i + 1) +  event_id_span' t1).
+    eapply IHt1.
+    2: { eassumption. }
+    econstructor; eauto.
+
+    assert (event_id_span' t2 = event_id_span (copland_compile t2)).
+    {
+      eapply event_id_spans_same.
+    }
+    
+    lia.
+Qed.
+
+
+  
+(** * CVM event ID span same as annotated term range *)
+Lemma span_cvm: forall atp t annt i j e e' tr tr' p p' i',
+    build_cvmP
+      atp
+      {| st_ev := e;
+         st_trace := tr;
+         st_pl := p;
+         st_evid := i |} 
+      (Some tt)
+      {| st_ev := e';
+         st_trace := tr';
+         st_pl := p';
+         st_evid := i' |} ->
+    
+    term_to_coreP t atp -> 
+    anno t i = (j, annt) ->
+    j = i'.
+Proof.
+  intros.
+  assert (j = i + event_id_span' t).
+  {
+    assert (j - i = event_id_span' t).
+    {
+      symmetry.
+      eapply span_range.
+      eauto.
+    }
+    rewrite <- H2.
+    assert (j > i).
+    {
+      eapply anno_mono; eauto.
+    }
+    lia.
+  }
+  subst.
+  symmetry.
+  eapply cvm_spans; eauto.
+Defined.
+
+
+(** * Propositional version of span_cvm *)
+Lemma anno_span_cvm: forall t pt annt i i' e e' p p' tr tr' st_evid1,
+    annoP_indexed annt t i i' ->
+    term_to_coreP t pt ->
+    build_cvmP pt
+                     {|
+                       st_ev := e ;
+                       st_trace := tr ;
+                       st_pl := p;
+                       st_evid := i
+                     |} (Some tt)
+                     {|
+                       st_ev := e';
+                       st_trace := tr';
+                       st_pl := p';
+                       st_evid := st_evid1
+                     |} ->
+    i' = st_evid1.
+Proof.
+  intros.
+  invc H.
+  eapply span_cvm; eauto.
+Qed.
+
+
+
+
+
+Lemma wfec_firstn: forall e0 e1 e2,
+    wf_ec (evc e0 e1) ->
+    firstn (et_size e1) (e0 ++ e2) = e0.
+Proof.
+  intros.
+  inv_wfec.
+  jkjke'.
+  eapply More_lists.firstn_append.
+Defined.
+
+Ltac do_wfec_firstn :=
+  match goal with
+  | [H: context[(firstn (et_size ?e1) (?e0 ++ ?e2))],
+        H2: wf_ec (evc ?e0 ?e1)
+
+     |- _] =>
+    
+    assert_new_proof_by
+      (firstn (et_size e1) (e0 ++ e2) = e0)
+      ltac: (eapply wfec_firstn; apply H2)
+  end.
+
+Lemma wfec_skipn: forall e0 e1 e2,
+    wf_ec (evc e0 e1) ->
+    skipn (et_size e1) (e0 ++ e2) = e2.
+Proof.
+  intros.
+  inv_wfec.
+  jkjke'.
+  eapply More_lists.skipn_append.
+Defined.
+
+Ltac do_wfec_skipn :=
+  match goal with
+  | [H: context[(skipn (et_size ?e1) (?e0 ++ ?e2))],
+        H2: wf_ec (evc ?e0 ?e1)
+
+     |- _] =>
+    
+    assert_new_proof_by
+      (skipn (et_size e1) (e0 ++ e2) = e2)
+      ltac: (eapply wfec_skipn; apply H2)
+  end.
+
+Ltac clear_skipn_firstn :=
+  match goal with
+  | [H: firstn _ _ = _,
+        H2: skipn _ _ = _ |- _]
+    => rewrite H in *; clear H;
+      rewrite H2 in *; clear H2
+  end.
+
+
+
+
+
+(** * Axiom:  assume parallel CVM threads preserve well-formedness of EvC bundles *)
+Axiom wf_ec_preserved_par: forall e l t2 p,
+    wf_ec e ->
+    wf_ec (parallel_vm_thread l t2 p e).
+
+(** * Lemma:  CVM execution preserves well-formedness of EvC bundles 
+      (Evidence Type of sufficient length for raw evidence). *)
+Lemma wf_ec_preserved_by_cvm : forall e e' t1 tr tr' p p' i i',
+    wf_ec e ->
+        build_cvmP t1
+                    {| st_ev := e; st_trace := tr; st_pl := p; st_evid := i |}
+                    (Some tt)
+                    {| st_ev := e'; st_trace := tr'; st_pl := p'; st_evid := i' |} ->
+    wf_ec (e').
+Proof.
+  intros.
+  generalizeEverythingElse t1.
+  induction t1; intros.
+  -
+    rewrite <- ccp_iff_cc in *.
+    destruct a; (* asp *)
+      try destruct a; (* asp params *)
+      ff;
+      inv_wfec;
+      try (
+          econstructor;
+          ff;
+          try tauto;
+          try congruence).
+    +
+      destruct f.
+      ++
+        ff.
+        econstructor.
+        ff.
+      ++
+        ff.
+        econstructor.
+        ff.
+      ++
+        ff.
+        econstructor.
+        ff.
+        (* 
+        congruence. *)
+      ++
+        ff.
+        econstructor.
+        ff.
+      ++
+        ff.
+        econstructor.
+        ff.
+        
+        
+  -
+    wrap_ccp.
+
+    eapply wf_ec_preserved_remote; eauto.
+
+  -
+    wrap_ccp.
+    eauto.
+  -
+    wrap_ccp.
+
+    (*
+
+    do_wfec_split. *)
+
+    find_apply_hyp_hyp.
+    find_apply_hyp_hyp.
+    econstructor.
+    dd.
+    inv_wfec.
+    repeat jkjke'.
+    eapply app_length.
+
+  -
+    wrap_ccp.
+
+    (*
+    
+    do_wfec_split. *)
+
+    find_apply_hyp_hyp.
+
+      inv_wfec;
+      ff;
+      econstructor;
+      dd;
+      repeat jkjke'.
+
+    erewrite app_length.
+
+    assert (wf_ec (evc r0 e1)).
+    {
+      rewrite <- Heqe1.
+      eapply wf_ec_preserved_par.
+      econstructor; eassumption.
+    }
+
+    solve_by_inversion.
+Qed.
+
+Ltac do_wfec_preserved :=
+  repeat
+    match goal with
+    | [(*H: well_formed_r ?t, *)
+          H2: wf_ec ?stev,
+              H3: build_cvmP ?t
+                                   {| st_ev := ?stev; st_trace := _; st_pl := _; st_evid := _ |}
+                                   (Some tt)
+                                   {| st_ev := ?stev'; st_trace := _; st_pl := _; st_evid := _ |}
+       |- _ ] =>
+      assert_new_proof_by (wf_ec stev')
+                          ltac:(eapply wf_ec_preserved_by_cvm; [(*apply H |*) apply H2 | apply H3])
+                                 
+    end.
+
+
+Axiom ev_cvm_mtc: forall ct p e loc,
+    parallel_vm_thread loc ct p mt_evc = parallel_vm_thread loc (lseqc (aspc CLEAR) ct) p e.
+
+
+
 (*
 TODO: try this lemma again after getting appraisal Lemmas settled 
+*)
 
 
 (** * Lemma:  relating reconstructed CVM EvC bundles via the EvidenceC evidence denotation. *)
@@ -1131,12 +1921,15 @@ Proof.
         wrap_ccp_anno.
         invc H3.
         ff.
+      ++ (* KILL case *)
+        wrap_ccp_anno.
+        invc H3.
+        ff.
       ++
-        admit.
-      ++
-        admit.
-        
-        
+        wrap_ccp_anno.
+        invc H3.
+        ff.
+             
       ++
         wrap_ccp_anno.
         invc H3.
@@ -1144,17 +1937,19 @@ Proof.
         assert (et_fun ec' = et').
         {
           symmetry.
-        eapply etfun_reconstruct.
+          eapply etfun_reconstruct.
+          econstructor.
+          
         eassumption.
         }
+        invc H2.
+        unfold reconstruct_ev in *.
         congruence.
       ++
         wrap_ccp_anno.
         invc H3.
         ff.
-        
-        
-        
+
     +
       dd.
       invc H3; invc H2.
@@ -2017,6 +2812,7 @@ Proof.
     +
       destruct f; ff.
       destruct s; ff.
+      destruct s; ff.
   -
     dd.
     eauto.
@@ -2035,7 +2831,6 @@ Proof.
     jkjke.
     destruct s; destruct s; destruct s0; eauto.
 Defined.
-*)
 
 
 
